Refine minimal_transition and lemmas about it

SafetyOracles.thy
@@ -20,7 +20,7 @@ fun from_sender :: "(validator * state) \<Rightarrow> message set"
 (* Definition 7.3 *)
 fun later_from :: "(message * validator * state) \<Rightarrow> message set"
   where
-    "later_from (m, v, \<sigma>) = {m'. m \<in> \<sigma> \<and> sender m' = v \<and> later (m', m)}"
+    "later_from (m, v, \<sigma>) = {m'. m' \<in> \<sigma> \<and> sender m' = v \<and> later (m', m)}"
  
 (* Definition 7.4 *)
 fun latest_messages :: "(state * validator) \<Rightarrow> message set"
@@ -100,33 +100,75 @@ fun is_clique :: "(validator set * consensus_value_property * state) \<Rightarro
 (* Definition 7.17 *)
 fun minimal_transitions :: "params \<Rightarrow> (state * state) set"
   where
-    "minimal_transitions params = {(\<sigma>, \<sigma>') | \<sigma> \<sigma>'. \<sigma> \<in> \<Sigma>t params \<and> \<sigma>' \<in> \<Sigma>t params \<and> is_future_state (\<sigma>, \<sigma>') \<and> \<sigma> \<noteq> \<sigma>'
-      \<and> (\<nexists> \<sigma>''. \<sigma>'' \<in> \<Sigma> params \<and> is_future_state (\<sigma>, \<sigma>'') \<and> is_future_state (\<sigma>'', \<sigma>') \<and> \<sigma> \<noteq> \<sigma>'' \<and> \<sigma>'' \<noteq> \<sigma>')}"
+    "minimal_transitions params = {(\<sigma>, \<sigma>') | \<sigma> \<sigma>'. \<sigma> \<in> \<Sigma>t params \<and> \<sigma>' \<in> \<Sigma>t params \<and> is_future_state (\<sigma>', \<sigma>) \<and> \<sigma> \<noteq> \<sigma>'
+      \<and> (\<nexists> \<sigma>''. \<sigma>'' \<in> \<Sigma> params \<and> is_future_state (\<sigma>'', \<sigma>) \<and> is_future_state (\<sigma>', \<sigma>'') \<and> \<sigma> \<noteq> \<sigma>'' \<and> \<sigma>'' \<noteq> \<sigma>')}"
+
+(* Temporary lemmas for minimal_transition_implies_recieving_a_single_message *)
+lemma no_intermidiate_implies_difference_is_singleton :
+  "\<forall> A B. A \<subseteq> B \<and> A \<noteq> B \<longrightarrow> (\<nexists> C. A \<subseteq> C \<and> C \<subseteq> B \<and> A \<noteq> C \<and> B \<noteq> C) \<longrightarrow> is_singleton (B - A)"    
+  apply simp
+  by (smt DiffD1 DiffD2 Diff_eq_empty_iff Diff_insert_absorb Diff_subset double_diff insert_subset is_singleton_def psubsetI psubset_imp_ex_mem)
+
+lemma difference_is_singleton_implies_no_intermidiate :
+  "\<forall> A B. A \<subseteq> B \<and> A \<noteq> B \<longrightarrow> is_singleton (B - A) \<longrightarrow> (\<nexists> C. A \<subseteq> C \<and> C \<subseteq> B \<and> A \<noteq> C \<and> B \<noteq> C)"
+  by (smt Diff_cancel Diff_eq_empty_iff Diff_insert0 double_diff insert_Diff is_singleton_def)
 
 lemma "set_difference_and_singleton" :
-  "\<forall> A B. A \<subseteq> B \<and> A \<noteq> B \<longrightarrow> (\<nexists> C. A \<subseteq> C \<and> C \<subseteq> B \<and> A \<noteq> C \<and> B \<noteq> C) \<longleftrightarrow> is_singleton (B - A)" 
-proof -
-  have right :
-    "\<forall> A B. A \<subseteq> B \<and> A \<noteq> B \<longrightarrow> (\<nexists> C. A \<subseteq> C \<and> C \<subseteq> B \<and> A \<noteq> C \<and> B \<noteq> C) \<longrightarrow> is_singleton (B - A)"    
-    apply simp
-    by (smt DiffE empty_iff insertCI insertE insert_Diff_if insert_subset is_singletonI' order_refl psubsetI psubset_imp_ex_mem set_diff_eq)
-  have left :
-    "\<forall> A B. A \<subseteq> B \<and> A \<noteq> B \<longrightarrow> is_singleton (B - A) \<longrightarrow> (\<nexists> C. A \<subseteq> C \<and> C \<subseteq> B \<and> A \<noteq> C \<and> B \<noteq> C)"
-    by (smt Diff_cancel Diff_eq_empty_iff Diff_insert0 double_diff insert_Diff is_singleton_def)
-  moreover show ?thesis
-    using right left by metis
-qed
+  "\<forall> A B. A \<subseteq> B \<and> A \<noteq> B \<longrightarrow> (\<nexists> C. A \<subseteq> C \<and> C \<subseteq> B \<and> A \<noteq> C \<and> B \<noteq> C) \<longleftrightarrow> is_singleton (B - A)"
+  using no_intermidiate_implies_difference_is_singleton difference_is_singleton_implies_no_intermidiate by metis
 
-lemma minimal_transition_corresponds_to_recieving_a_single_message :
+lemma no_intermidiate_implies_difference_is_singleton_with_set :
+  "\<forall> \<sigma> \<sigma>' M. \<sigma> \<in> Pow M \<and> \<sigma>' \<in> Pow M 
+  \<longrightarrow> \<sigma> \<subseteq> \<sigma>' \<and> \<sigma> \<noteq> \<sigma>' 
+  \<longrightarrow> (\<nexists> \<sigma>''. \<sigma>'' \<in> Pow M \<and> \<sigma> \<subseteq> \<sigma>'' \<and> \<sigma>'' \<subseteq> \<sigma>' \<and> \<sigma> \<noteq> \<sigma>'' \<and> \<sigma>''\<noteq> \<sigma>')
+  \<longrightarrow> is_singleton {m. m \<in> M \<inter> \<sigma>'- \<sigma>}"
+  by (metis Collect_mem_eq Int_absorb2  Pow_iff inf_commute no_intermidiate_implies_difference_is_singleton subset_trans)
+
+lemma state_difference_is_valid_message :
+  "\<forall> params \<sigma> \<sigma>'. is_valid_params params \<and> \<sigma> \<in> \<Sigma> params \<and> \<sigma>' \<in> \<Sigma> params
+  \<longrightarrow> is_future_state(\<sigma>', \<sigma>)
+  \<longrightarrow> \<sigma>' - \<sigma> \<subseteq> M params"
+  apply (simp add: \<Sigma>_def M_def)
+sorry
+
+lemma "A \<subseteq> B \<and> is_singleton {a. a \<in> A \<inter> B} \<longrightarrow> is_singleton A"
+  by (metis Collect_mem_eq inf.orderE)
+
+(* A minimal transition corresponds to recieving a single new message with justification drawn from the initial
+protocol state *)
+lemma minimal_transition_implies_recieving_a_single_message :
   "\<forall> params \<sigma> \<sigma>'. is_valid_params params \<and> \<sigma> \<in> \<Sigma>t params \<and> \<sigma>' \<in> \<Sigma>t params
-  \<longrightarrow> (\<sigma>, \<sigma>') \<in> minimal_transitions params \<longleftrightarrow> is_singleton (\<sigma>' - \<sigma>)"
+  \<longrightarrow> (\<sigma>, \<sigma>') \<in> minimal_transitions params \<longrightarrow> is_singleton (\<sigma>'- \<sigma>)"
+proof -
+  have lemma1 :
+    "\<forall> params \<sigma> \<sigma>'. is_valid_params params \<and> \<sigma> \<in> \<Sigma>t params \<and> \<sigma>' \<in> \<Sigma>t params
+    \<longrightarrow> (\<sigma>, \<sigma>') \<in> minimal_transitions params \<longrightarrow> is_singleton (M params \<inter> \<sigma>'- \<sigma>)"
+  proof -
+    have minimal_transition_implies_no_intermidiate :
+      "\<forall> params \<sigma> \<sigma>'. is_valid_params params \<and> \<sigma> \<in> \<Sigma>t params \<and> \<sigma>' \<in> \<Sigma>t params
+      \<longrightarrow> (\<sigma>, \<sigma>') \<in> minimal_transitions params 
+      \<longrightarrow> \<sigma> \<subseteq> \<sigma>' \<and> \<sigma> \<noteq> \<sigma>' \<and> (\<nexists> \<sigma>''. \<sigma>'' \<in> \<Sigma> params \<and> \<sigma> \<subseteq> \<sigma>'' \<and> \<sigma>'' \<subseteq> \<sigma>' \<and> \<sigma> \<noteq> \<sigma>'' \<and> \<sigma>''\<noteq> \<sigma>')"
+      by simp
+    have no_intermidiate_implies_single_message :
+      "\<forall> params \<sigma> \<sigma>'. is_valid_params params \<and> \<sigma> \<in> \<Sigma>t params \<and> \<sigma>' \<in> \<Sigma>t params 
+      \<longrightarrow> \<sigma> \<subseteq> \<sigma>' \<and> \<sigma> \<noteq> \<sigma>' 
+      \<longrightarrow> (\<nexists> \<sigma>''. \<sigma>'' \<in> \<Sigma> params \<and> \<sigma> \<subseteq> \<sigma>'' \<and> \<sigma>'' \<subseteq> \<sigma>' \<and> \<sigma> \<noteq> \<sigma>'' \<and> \<sigma>''\<noteq> \<sigma>')
+      \<longrightarrow> is_singleton (M params \<inter> \<sigma>'- \<sigma>)"
+      (* TODO  *)
+      sorry
+    moreover show ?thesis
+      sorry  
+  have lemma2 : 
+    "\<forall> params \<sigma> \<sigma>'. is_valid_params params \<and> \<sigma> \<in> \<Sigma>t params \<and> \<sigma>' \<in> \<Sigma>t params
+    \<longrightarrow> is_singleton {m \<in> M params \<inter> \<sigma>'- \<sigma>} \<longrightarrow> is_singleton (\<sigma>' - \<sigma>)"
+    using state_difference_is_valid_message
   oops
 
-(* Lemma 11: Minimal transitions do not change Later From for any non-sender *)
+(* Lemma 11: Minimal transitions do not change Later_From for any non-sender *)
 lemma later_from_not_affected_by_minimal_transitions :
-  "\<forall> params \<sigma> \<sigma>' m. is_valid_params params \<and> (\<sigma>, \<sigma>') \<in> minimal_transitions params \<and> m \<in> M params
-  \<longrightarrow> (\<forall> v. v \<in> V params - {sender (the_elem {m'. m \<in> \<sigma>' - \<sigma>})} \<longrightarrow> later_from (m, v, \<sigma>) = later_from (m, v, \<sigma>'))"
-  (* TODO *)
+  "\<forall> params \<sigma> \<sigma>' m. is_valid_params params \<and> (\<sigma>, \<sigma>') \<in> minimal_transitions params
+  \<longrightarrow> m = the_elem (\<sigma>' - \<sigma>)
+  \<longrightarrow> (\<forall> v \<in> V params - {sender m}. later_from (m, v, \<sigma>) = later_from (m, v, \<sigma>'))"
   oops
 
 end
